Composition of context coercions and attempt at SubstCtxConv translation

formalization/ctt.v
@@ -92,33 +92,39 @@ Definition substCoerce : Type :=
   contextCoercion * contextCoercion.
 
 (* Inverses of coercions *)
-Definition contextInv c : contextCoercion :=
-  {| ctxco_map := ctxco_inv c
-   ; ctxco_inv := ctxco_map c |}.
+(* We'll put them back if ever needed (most probable).
+   In this event, we will probably need to enrich the definition. *)
+(* Definition contextInv c : contextCoercion := *)
+(*   {| ctxco_map := ctxco_inv c *)
+(*    ; ctxco_inv := ctxco_map c |}. *)
 
-Lemma ctx_inverse :
-  forall {c G D}, isContextCoercion c G D ->
-             isContextCoercion (contextInv c) D G.
-Proof.
-  intros c G D H.
-  destruct H as [[h1 h2] h3].
-  repeat split.
-  - assumption.
-  - assumption.
-  - intros A u H.
-    pose (sbs := ctxco_inv c).
-    pose (As := itt.Subst A sbs).
-    pose (us := itt.subst u sbs).
-    assert (H' : itt.isterm D us As).
-    { eapply itt.TermSubst.
-      - exact h2.
-      - assumption.
-    }
-    destruct (h3 As us H') as (p & Hp).
-    (* Am I missing something? Or do we need to modify the definition? *)
-    admit.
-Admitted.
+(* Lemma ctx_inverse : *)
+(*   forall {c G D}, isContextCoercion c G D -> *)
+(*              isContextCoercion (contextInv c) D G. *)
+(* Proof. *)
+(*   intros c G D H. *)
+(*   destruct H as [[h1 h2] h3]. *)
+(*   repeat split. *)
+(*   - assumption. *)
+(*   - assumption. *)
+(*   - intros A u H. *)
+(*     pose (sbs := ctxco_inv c). *)
+(*     pose (As := itt.Subst A sbs). *)
+(*     pose (us := itt.subst u sbs). *)
+(*     assert (H' : itt.isterm D us As). *)
+(*     { eapply itt.TermSubst. *)
+(*       - exact h2. *)
+(*       - assumption. *)
+(*     } *)
+(*     destruct (h3 As us H') as (p & Hp). *)
+(*     (* Am I missing something? Or do we need to modify the definition? *) *)
+(*     admit. *)
+(* Admitted. *)
 
+(* Composition of coercions *)
+Definition contextComp c1 c2 : contextCoercion :=
+  {| ctxco_map := itt.sbcomp (ctxco_map c1) (ctxco_map c2)
+   ; ctxco_inv := itt.sbcomp (ctxco_inv c2) (ctxco_inv c1) |}.
 
 
 Definition typeInv c : typeCoercion :=
